CCAS WIP

examples/CCAS.v
@@ -21,6 +21,13 @@ Require Import Specs.
 Require Import SeparationAlgebra.
 
 
+  Lemma conj_from_imp : forall (P Q : Prop), P -> (P -> Q) -> P /\ Q.
+  Proof. eauto. Qed.
+  
+  Lemma conj_right_imp {P Q R : Prop} :
+    (Q -> R) -> (P /\ Q) -> (P /\ R).
+  Proof. tauto. Qed.
+
   Ltac split_right :=
     try (split; [| split_right]).
 
@@ -47,8 +54,7 @@ Class HasBeq (t : Type) := {
   beq_false : forall x y, beq x y = false -> x <> y;
 }.
 
-(* TODO: change IsExpired to owner *)
-(* Module CASTaskImpl.
+Module CASTaskImpl.
   Import LinCCALBase.
   Import LTSSpec.
   Import Lang.
@@ -77,7 +83,7 @@ Class HasBeq (t : Type) := {
   {|
     li_sig := ECASTask Val;
     li_lts := VCASTask;
-    li_init := Idle (cts (inr vInit) O nil);
+    li_init := Idle (cts (inr vInit) O (fun _ => Inactive));
   |}.
 
   Definition allocTask_impl (_ : tid) : Prog (li_sig E) nat :=
@@ -88,7 +94,601 @@ Class HasBeq (t : Type) := {
   
   Definition tryResolveTask_impl tsk v (_ : tid) : Prog (li_sig E) unit :=
     inl (cas (inl tsk) (inr v)) >= _ => Ret tt.
-End CASTaskImpl. *)
+  
+  Definition assertion := @Assertion (@ProofState _ _ (li_lts E) (li_lts F)).
+  Definition rg_relation := @RGRelation _ _ (li_lts E) (li_lts F).
+
+  Open Scope rg_relation_scope.
+  Open Scope assertion_scope.
+  
+  Definition ALinEx t ls : assertion := fun s => exists ρ π, Δ s ρ π /\ TMap.find t π = ls.
+
+  Definition I_cas : assertion := fun s =>
+    forall ρ π, Δ s ρ π ->
+      state (fst (σ s)) = current (state ρ).
+
+  Definition I_ticket : assertion := fun s =>
+    forall ρ π, Δ s ρ π ->
+      state (snd (σ s)) = ticket (state ρ) /\
+      forall i, ticket (state ρ) <= i -> owner (state ρ) i = Inactive.
+
+  Definition I_atomic : assertion := fun s =>
+    exists ρ π c, Δ s ≡ [(ρ , π)] /\ ρ = Idle c.
+    
+  Definition I : assertion :=
+    I_atomic //\\ I_cas //\\ I_ticket.
+  
+  Definition R t : rg_relation :=
+    fun s1 s2 =>
+      forall ls, ALinEx t ls s1 <-> ALinEx t ls s2.
+  
+  Definition G_id : rg_relation :=
+    fun s1 s2 =>
+      state (fst (σ s1)) = state (fst (σ s2)) /\
+      state (snd (σ s1)) = state (snd (σ s2)) /\
+      Δ s1 ≡ Δ s2.
+
+  Definition G_other t : rg_relation :=
+    fun s1 s2 => forall t', t <> t' -> R t' s1 s2.
+  
+  Definition G t := G_id ∪ G_other t.
+
+  Ltac simpl_all :=
+    unfold R, G, G_id, G_other, I, I_atomic, I_ticket, I_cas,
+          Conj, Disj, Imply in *; simpl in *.
+
+  Lemma RG_compatible : forall t1 t2, t1 <> t2 -> (I ⊓ G t1 ⊆ R t2).
+  Proof.
+    intros. intros ? ? [? ?].
+    destruct H0.
+    - unfold G_id, R, ALinEx in *.
+      split; intros [? [? [HΔ ?]]];
+      apply H0 in HΔ; do 2 eexists; eauto.
+    - apply H0; eauto.
+  Qed.
+
+  Lemma R_domexact : forall t0 s1 s2, R t0 s1 s2 -> I s2 ->
+    (forall (ρ1 : State (li_lts F)) (π1 : tmap LinState), Δ s1 ρ1 π1 -> TMap.find t0 π1 = None) <->
+    (forall (ρ2 : State (li_lts F)) (π2 : tmap LinState), Δ s2 ρ2 π2 -> TMap.find t0 π2 = None).
+  Proof.
+    intros.
+    split; intros.
+    - pose proof ac_nonempty (Δ s1) as [? [? ?]].
+      apply H1 in H3 as ?.
+      assert (ALinEx t0 None s1) by (do 2 eexists; eauto).
+      apply H in H5 as [? [? [? ?]]].
+      eapply (ac_domexact (Δ s2)) in H6; eauto.
+    - pose proof ac_nonempty (Δ s2) as [? [? ?]].
+      apply H1 in H3 as ?.
+      assert (ALinEx t0 None s2) by (do 2 eexists; eauto).
+      apply H in H5 as [? [? [? ?]]].
+      eapply (ac_domexact (Δ s1)) in H6; eauto.
+  Qed.
+
+  Lemma ALinLinExI : forall t ls s,
+    I s -> (ALinEx t (Some ls) s <-> ALin t ls s).
+  Proof.
+    intros. destruct H as [[? [? [? [? ?]]]]].
+    split; intros.
+    - intros ? ? ?. apply H in H3; inversion H3; subst.
+      destruct H2 as [? [? [? ?]]].
+      apply H in H0; inversion H0; subst. auto.
+    - exists x, x0. split; [apply H; constructor|].
+      pose proof ac_nonempty (Δ s) as [? [? ?]].
+      apply H in H3; inversion H3; subst.
+      eapply H2. apply H; eauto.
+  Qed.
+
+  Lemma ALinLinEx : forall t ls s,
+    ALin t ls s -> ALinEx t (Some ls) s.
+  Proof.
+    intros.
+    pose proof ac_nonempty (Δ s) as [? [? ?]].
+    apply H in H0 as ?. do 2 eexists; eauto.
+  Qed.
+
+  Lemma stable_ALin : forall t ls, Stable (R t) I (ALin t ls).
+  Proof.
+    intros. intros ? [[? [? ?]] ?].
+    rewrite <- ALinLinExI; eauto. apply H0.
+    apply ALinLinEx; auto.
+  Qed.
+
+  Lemma stable_I : forall t, Stable (R t) I I.
+  Proof. intros. intros ? [[? [? ?]] ?]; auto. Qed.
+
+  Lemma G_id_I : ⊨ G_id ⊚ I ==>> I.
+  Proof.
+    intros ? [? [? [? [? ?]]]].
+    destruct H as [[? [? [? [? ?]]]] [? ?]]; subst.
+    simpl_all. rewrite H0 in *. rewrite H1 in *.
+    split; [|split]; eauto.
+    - exists (Idle x2), x1, x2.
+      split; auto. etransitivity; eauto. symmetry; auto.
+    - intros. apply H2 in H3; eauto.
+    - intros. apply H2 in H3; eauto.
+  Qed.
+
+  Create HintDb stableDB.
+  Hint Resolve stable_I stable_ALin
+  : stableDB.
+
+  Lemma G_id_G : forall s1 s2 t, G_id s1 s2 -> G t s1 s2.
+  Proof. left; auto. Qed.
+  
+  Ltac post_pupdate_id :=
+            eapply conj_right_imp; [apply G_id_G |];
+                    apply and_comm, conj_from_imp; intros.
+
+  Program Definition MCASTask : layer_implementation E F := {|
+    li_impl m :=
+      match m with
+      | allocTask _ _ => allocTask_impl
+      | tryPlaceTask o n i => tryPlaceTask_impl o n i
+      | tryResolveTask tsk v => tryResolveTask_impl tsk v
+      end
+  |}.
+  Next Obligation.
+    eapply RGILogic.soundness with (R:=R) (G:=G) (I:=I).
+    (* valid RG *)
+    {
+      constructor.
+      apply R_domexact.
+    }
+    {
+      intros. intros s1 s2 [[? | ?] HI];
+      [eapply RG_compatible; eauto; try (split; auto)|].
+      destruct H0 as [[? | ?] | ?].
+      - unfold GINV, Ginv, LiftRelation_Δ in *.
+        destruct H0 as [? [? [? ?]]].
+        split; intros [? [? [? ?]]].
+        + exists x0, (TMap.add t1 (ls_inv x) x1).
+          split; [|rewrite TMap.gso;auto].
+          apply H2. constructor; auto.
+        + apply H2 in H3. inversion H3; subst.
+          do 2 eexists; split; eauto.
+          rewrite TMap.gso; auto.
+      - unfold GRET, Gret, LiftRelation_Δ in *.
+        destruct H0 as [? [? [? [? ?]]]].
+        split; intros [? [? [? ?]]].
+        + exists x1, (TMap.remove t1 x2).
+          split; [|rewrite TMap.gro;auto].
+          apply H2. constructor; auto.
+        + apply H2 in H3. inversion H3; subst.
+          do 2 eexists; split; eauto.
+          rewrite TMap.gro; auto.
+      - unfold GId in *; subst. unfold R. tauto.
+    }
+    (* method provable *)
+    {
+      intros t f.
+      exists (I //\\ ALin t (ls_inv f)).
+      exists (fun r => I //\\ ALin t (ls_linr f r)).
+      constructor;
+      try solve_conj_impl;
+      try solve_stable stableDB.
+      (* invocation *)
+      {
+        intros ? [s' [? [? [? ?]]]]. simpl_all.
+        rewrite H0 in *.
+        destruct H as [[? [? [? [? ?]]]] [? ?]]; subst.
+        split;[split;[|split]|].
+        - exists (Idle x1), (TMap.add t (ls_inv f) x0).
+          exists x1; split; auto.
+          etransitivity; eauto.
+          split; inversion 1; subst; try constructor; eauto.
+          + apply H in Hposs; inversion Hposs; subst; auto.
+            constructor.
+          + apply H. constructor.
+        - intros. apply H2 in H3; inversion H3; subst. eauto.
+        - intros. apply H2 in H3. inversion H3; subst. eauto.
+        - intros ? ? ?. apply H2 in H3; inversion H3; subst.
+          rewrite TMap.gss; eauto.
+      }
+      (* response *)
+      {
+        intros ? ? [? [[? ?] [? [? ?]]]]. simpl_all.
+        rewrite H1 in *.
+        destruct H as [[? [? [? [? ?]]]] [? ?]]; subst.
+        split;[|split].
+        - exists (Idle x2), (TMap.remove t x1).
+          exists x2; split; auto.
+          etransitivity; eauto.
+          split; inversion 1; subst; try constructor; eauto.
+          + apply H in Hposs; inversion Hposs; subst; auto.
+            constructor.
+          + apply H. constructor.
+        - intros. apply H3 in H4; inversion H4; subst. eauto.
+        - intros. apply H3 in H4; inversion H4; subst. eauto.
+      }
+      {
+        intros. destruct H as [_ ?]. eauto.
+      }
+      (* method body *)
+      {
+        destruct f.
+        (* alloc *)
+        {
+          simpl.
+          eapply provable_vis_safe with
+            (P' := I //\\ ALin t (ls_inv (allocTask o n)))
+            (Q' := fun r : nat => I //\\ ALin t (ls_linr (allocTask o n) r));
+          try solve_no_error;
+          try solve_conj_impl;
+          try solve_stable stableDB.
+          (* inv *)
+          {
+            pupdate_intros_atomic.
+            dependent destruction Hstep.
+            pupdate_start. eapply ac_steps_refl.
+            
+            post_pupdate_id.
+            { unfold G_id; simpl; do 2 (split; auto); reflexivity. }
+            destruct Hpre as [? ?].
+            split; [apply G_id_I; eexists; eauto|].
+            intros ? ? ?.
+            apply H1 in H2. auto.
+          }
+          (* res *)
+          {
+            pupdate_intros_atomic.
+            dependent destruction Hstep.
+            destruct Hpre as [? ?].
+            pose proof ac_nonempty (Δ1) as [? [? ?]].
+            apply H0 in H1 as ?.
+            destruct H as [[? [? [? [? ?]]]] ?].
+            apply H in H1 as HΔ; inversion HΔ; subst. simpl in *.
+            destruct x3.
+
+            pupdate_start.
+            pupdate_trylin_from H1.
+            pupdate_forward t (InvEv (allocTask o n)).
+            pupdate_forward t (ResEv (allocTask o n) ticket0).
+            pupdate_finish.
+            eapply ACTrylinFinish.
+
+            repeat split; simpl_all.
+            - exists (Idle {| current := current0; ticket := S ticket0; owner := owner_upd owner0 ticket0 (Owned t) |}).
+              exists (TMap.add t (ls_linr (allocTask o n) ticket0) (TMap.add t (ls_lini (allocTask o n)) x0)).
+              eexists; split; [|split;eauto].
+              constructor; inversion 1; subst; try constructor; eauto.
+              pupdate_forward t (InvEv (allocTask o n)).
+              pupdate_forward t (ResEv (allocTask o n) ticket0).
+              pupdate_finish.
+            - inversion 1; subst. simpl in *.
+              destruct H4.
+              apply H4 in H1. eauto.
+            - inversion H3; subst. simpl. apply f_equal.
+              apply H4 in H1 as [? ?]. eauto.
+            - inversion H3; subst. simpl.
+              apply H4 in H1 as [? ?]. simpl in *.
+              intros. unfold owner_upd.
+              destruct (Nat.eqb_spec ticket0 i); subst; eauto; try lia.
+              eapply H5. lia.
+            - inversion 1; subst. simpl_all.
+              rewrite TMap.gss; eauto.
+              apply H4 in Hposs as [? ?]; simpl in *. subst. eauto.
+            - right. intros. simpl_all.
+              split; intros [? [? [? ?]]]; [|inversion H5;subst].
+              + exists (Idle {| current := current0; ticket := S ticket0; owner := owner_upd owner0 ticket0 (Owned t) |}),
+                (TMap.add t (ls_linr (allocTask o n) ticket0) (TMap.add t (ls_lini (allocTask o n)) x0)).
+                apply H in H5 as HΔ'; inversion HΔ'; simpl in *; subst.
+                simpl. split; [constructor|do 2 (rewrite TMap.gso; eauto) ]; eauto.
+                pupdate_forward t (InvEv (allocTask o n)).
+                pupdate_forward t (ResEv (allocTask o n) ticket0).
+                pupdate_finish.
+              + exists (Idle {| current := current0; ticket := ticket0; owner := owner0 |}), x0. split; eauto.
+                do 2 (rewrite TMap.gso; eauto).
+          }
+          intros.
+          eapply provable_ret;
+          try solve_conj_impl;
+          try solve_stable stableDB.
+          left; auto.
+        }
+        (* place *)
+        {
+          simpl.
+          eapply provable_vis_safe with
+            (P' := I //\\ ALin t (ls_inv (tryPlaceTask o n i)))
+            (Q' := fun r => I //\\ ALin t (ls_linr (tryPlaceTask o n i) r));
+          try solve_no_error;
+          try solve_conj_impl;
+          try solve_stable stableDB.
+          (* inv *)
+          {
+            pupdate_intros_atomic.
+            dependent destruction Hstep.
+            pupdate_start. eapply ac_steps_refl.
+            
+            post_pupdate_id.
+            { unfold G_id; simpl; do 2 (split; auto); reflexivity. }
+            destruct Hpre as [? ?].
+            split; [apply G_id_I; eexists; eauto|].
+            intros ? ? ?.
+            apply H1 in H2. auto.
+          }
+          (* res *)
+          {
+            pupdate_intros_atomic;
+            dependent destruction Hstep.
+            (* succeed *)
+            {
+              destruct Hpre as [? ?].
+              pose proof ac_nonempty (Δ1) as [? [? ?]].
+              apply H0 in H1 as ?.
+              destruct H as [[? [? [? [? ?]]]] ?].
+              apply H in H1 as HΔ; inversion HΔ; subst. simpl in *.
+              destruct x3.
+              pose proof H4 as [? _]. apply H3 in H1 as ?; simpl in *. subst.
+
+              pupdate_start.
+              pupdate_trylin_from H1.
+              eapply rt_trans.
+              eapply rt_step, ps_inv; eauto.
+              do 2 constructor.
+              eapply rt_step, ps_ret; eauto.
+              constructor. eapply step_tryPlaceTask_succ; eauto.
+              rewrite TMap.gss; auto.
+              eapply ACTrylinFinish.
+
+              repeat split; simpl_all.
+              - exists (Idle {| current := inl (CTask t0 o n i); ticket := ticket0; owner := owner0 |}),
+                (TMap.add t0 (ls_linr (tryPlaceTask o n i) (inr o)) (TMap.add t0 (ls_lini (tryPlaceTask o n i)) x0)).
+                eexists; split; [|split;eauto].
+                constructor; inversion 1; subst; try constructor; eauto.
+                eapply rt_trans.
+                eapply rt_step, ps_inv; eauto.
+                do 2 constructor.
+                eapply rt_step, ps_ret; eauto.
+                constructor. eapply step_tryPlaceTask_succ; eauto.
+                rewrite TMap.gss; auto.
+              - inversion 1; subst. simpl in *.
+                destruct H4.
+                apply H4 in H1. eauto.
+              - inversion H5; subst. simpl.
+                apply H4 in H1 as [? ?]. eauto.
+              - inversion H5; subst. simpl.
+                apply H4 in H1 as [? ?]. simpl in *.
+                intros. unfold owner_upd.
+                destruct (Nat.eqb_spec ticket0 i); subst; eauto; try lia.
+              - inversion 1; subst. simpl_all.
+                rewrite TMap.gss; eauto.
+              - right. intros. simpl_all.
+                split; intros [? [? [? ?]]]; [|inversion H6;subst].
+                + exists (Idle {| current := inl (CTask t0 o n i); ticket := ticket0; owner := owner0 |}),
+                    (TMap.add t0 (ls_linr (tryPlaceTask o n i) (inr o)) (TMap.add t0 (ls_lini (tryPlaceTask o n i)) x0)).
+                  apply H in H6 as HΔ'; inversion HΔ'; simpl in *; subst.
+                  simpl. split; [constructor|do 2 (rewrite TMap.gso; eauto) ]; eauto.
+                  eapply rt_trans.
+                  eapply rt_step, ps_inv; eauto.
+                  do 2 constructor.
+                  eapply rt_step, ps_ret; eauto.
+                  constructor. eapply step_tryPlaceTask_succ; eauto.
+                  rewrite TMap.gss; auto.
+                + do 2 eexists; split; eauto.
+                  do 2 (rewrite TMap.gso; eauto).
+            }
+            (* fail *)
+            {
+              clear H0. rename H1 into Hneq.
+              destruct Hpre as [? ?].
+              pose proof ac_nonempty (Δ1) as [? [? ?]].
+              apply H0 in H1 as ?.
+              destruct H as [[? [? [? [? ?]]]] ?]. subst.
+              apply H in H1 as HΔ; inversion HΔ; subst. simpl in *.
+              destruct x3.
+              pose proof H4 as [? _]. apply H3 in H1 as ?; simpl in *. subst.
+              destruct current0.
+              (* fail *)
+              {
+                pupdate_start.
+                pupdate_trylin_from H1.
+                eapply rt_trans.
+                eapply rt_step, ps_inv; eauto.
+                do 2 constructor.
+                eapply rt_step, ps_ret; eauto.
+                constructor. eapply step_tryPlaceTask_block; eauto.
+                rewrite TMap.gss; auto.
+                eapply ACTrylinFinish.
+
+                repeat split; simpl_all.
+                - exists (Idle {| current := inl c; ticket := ticket0; owner := owner0 |}),
+    (TMap.add t0 (ls_linr (tryPlaceTask o n i) (inl c)) (TMap.add t0 (ls_lini (tryPlaceTask o n i)) x0)).
+                  eexists; split; [|split;eauto].
+                  constructor; inversion 1; subst; try constructor; eauto.
+                  eapply rt_trans.
+                  eapply rt_step, ps_inv; eauto.
+                  do 2 constructor.
+                  eapply rt_step, ps_ret; eauto.
+                  constructor. eapply step_tryPlaceTask_block; eauto.
+                  rewrite TMap.gss; auto.
+                - inversion 1; subst. simpl in *.
+                  destruct H4.
+                  apply H4 in H1. eauto.
+                - inversion H5; subst. simpl.
+                  apply H4 in H1 as [? ?]. eauto.
+                - inversion H5; subst. simpl.
+                  apply H4 in H1 as [? ?]. simpl in *.
+                  intros. unfold owner_upd.
+                  destruct (Nat.eqb_spec ticket0 i); subst; eauto; try lia.
+                - inversion 1; subst. simpl_all.
+                  rewrite TMap.gss; eauto.
+                - right. intros. simpl_all.
+                  split; intros [? [? [? ?]]]; [|inversion H6;subst].
+                  + exists (Idle {| current := inl c; ticket := ticket0; owner := owner0 |}),
+    (TMap.add t0 (ls_linr (tryPlaceTask o n i) (inl c)) (TMap.add t0 (ls_lini (tryPlaceTask o n i)) x0)).
+                    apply H in H6 as HΔ'; inversion HΔ'; simpl in *; subst.
+                    simpl. split; [constructor|do 2 (rewrite TMap.gso; eauto) ]; eauto.
+                    eapply rt_trans.
+                    eapply rt_step, ps_inv; eauto.
+                    do 2 constructor.
+                    eapply rt_step, ps_ret; eauto.
+                    constructor. eapply step_tryPlaceTask_block; eauto.
+                    rewrite TMap.gss; auto.
+                  + do 2 eexists; split; eauto.
+                    do 2 (rewrite TMap.gso; eauto).
+              }
+              (* fail *)
+              {
+                assert (Hneq' : v <> o) by congruence.
+                pupdate_start.
+                pupdate_trylin_from H1.
+                eapply rt_trans.
+                eapply rt_step, ps_inv; eauto.
+                do 2 constructor.
+                eapply rt_step, ps_ret; eauto.
+                constructor. eapply step_tryPlaceTask_fail; eauto.
+                rewrite TMap.gss; auto.
+                eapply ACTrylinFinish.
+
+                repeat split; simpl_all.
+                - exists (Idle {| current := inr v; ticket := ticket0; owner := owner0 |}),
+    (TMap.add t0 (ls_linr (tryPlaceTask o n i) (inr v)) (TMap.add t0 (ls_lini (tryPlaceTask o n i)) x0)).
+                  eexists; split; [|split;eauto].
+                  constructor; inversion 1; subst; try constructor; eauto.
+                  eapply rt_trans.
+                  eapply rt_step, ps_inv; eauto.
+                  do 2 constructor.
+                  eapply rt_step, ps_ret; eauto.
+                  constructor. eapply step_tryPlaceTask_fail; eauto.
+                  rewrite TMap.gss; auto.
+                - inversion 1; subst. simpl in *.
+                  destruct H4.
+                  apply H4 in H1. eauto.
+                - inversion H5; subst. simpl.
+                  apply H4 in H1 as [? ?]. eauto.
+                - inversion H5; subst. simpl.
+                  apply H4 in H1 as [? ?]. simpl in *.
+                  intros. unfold owner_upd.
+                  destruct (Nat.eqb_spec ticket0 i); subst; eauto; try lia.
+                - inversion 1; subst. simpl_all.
+                  rewrite TMap.gss; eauto.
+                - right. intros. simpl_all.
+                  split; intros [? [? [? ?]]]; [|inversion H6;subst].
+                  + exists (Idle {| current := inr v; ticket := ticket0; owner := owner0 |}),
+    (TMap.add t0 (ls_linr (tryPlaceTask o n i) (inr v)) (TMap.add t0 (ls_lini (tryPlaceTask o n i)) x0)).
+                    apply H in H6 as HΔ'; inversion HΔ'; simpl in *; subst.
+                    simpl. split; [constructor|do 2 (rewrite TMap.gso; eauto) ]; eauto.
+                    eapply rt_trans.
+                    eapply rt_step, ps_inv; eauto.
+                    do 2 constructor.
+                    eapply rt_step, ps_ret; eauto.
+                    constructor. eapply step_tryPlaceTask_fail; eauto.
+                    rewrite TMap.gss; auto.
+                  + do 2 eexists; split; eauto.
+                    do 2 (rewrite TMap.gso; eauto).
+              }
+            }
+          }
+          intros.
+          eapply provable_ret;
+          try solve_conj_impl;
+          try solve_stable stableDB.
+          left; auto.
+        }
+        (* resolve *)
+        {
+          simpl.
+          eapply provable_vis_safe with
+            (P' := I //\\ ALin t (ls_inv (tryResolveTask tsk v)))
+            (Q' := fun _ => I //\\ ALin t (ls_linr (tryResolveTask tsk v) tt));
+          try solve_no_error;
+          try solve_conj_impl;
+          try solve_stable stableDB.
+          (* inv *)
+          {
+            pupdate_intros_atomic.
+            dependent destruction Hstep.
+            pupdate_start. eapply ac_steps_refl.
+            
+            post_pupdate_id.
+            { unfold G_id; simpl; do 2 (split; auto); reflexivity. }
+            destruct Hpre as [? ?].
+            split; [apply G_id_I; eexists; eauto|].
+            intros ? ? ?.
+            apply H1 in H2. auto.
+          }
+          (* res *)
+          {
+            pupdate_intros_atomic;
+            dependent destruction Hstep.
+            (* succeed *)
+            {
+              destruct Hpre as [? ?].
+              pose proof ac_nonempty (Δ1) as [? [? ?]].
+              apply H0 in H1 as ?.
+              destruct H as [[? [? [? [? ?]]]] ?].
+              apply H in H1 as HΔ; inversion HΔ; subst. clear HΔ. simpl in *.
+              destruct x3.
+              destruct tsk.
+              assert (current0 = inl (CTask t1 o n i) \/ current0 <> inl (CTask t1 o n i)) by apply classic.
+              destruct H3 as [? | Hneq]; subst.
+
+              {
+                pupdate_start.
+                pupdate_trylin_from H1.
+                eapply rt_trans.
+                eapply rt_step, ps_inv; eauto.
+                do 2 constructor.
+                eapply rt_step, ps_ret; eauto; [|rewrite TMap.gss; auto].
+                constructor. eapply step_tryResolveTask_succ; eauto.
+                eapply ACTrylinFinish.
+
+                repeat split; simpl_all.
+                - exists (Idle {| current := inr v; ticket := ticket0; owner := owner_upd owner0 i Expired |}),
+    (TMap.add t0 (ls_linr (tryResolveTask (CTask t1 o n i) v) tt)
+       (TMap.add t0 (ls_lini (tryResolveTask (CTask t1 o n i) v)) x0)).
+                  eexists; split; [|split;eauto].
+                  constructor; inversion 1; subst; try constructor; eauto.
+                  eapply rt_trans.
+                  eapply rt_step, ps_inv; eauto.
+                  do 2 constructor.
+                  eapply rt_step, ps_ret; eauto; [|rewrite TMap.gss; auto].
+                  constructor. eapply step_tryResolveTask_succ; eauto.
+                - inversion 1; subst. simpl in *.
+                  destruct H4.
+                  apply H4 in H1. eauto.
+                - inversion H3; subst. simpl.
+                  apply H4 in H1 as [? ?]. eauto.
+                - inversion H3; subst. simpl.
+                  apply H4 in H1 as [? ?]. simpl in *.
+                  intros. unfold owner_upd.
+                  (* FIXME: what if the user resolves a task with id larger than ticket *)
+                  destruct (Nat.eqb_spec ticket0 i); subst; eauto; try lia.
+                - inversion 1; subst. simpl_all.
+                  rewrite TMap.gss; eauto.
+                - right. intros. simpl_all.
+                  split; intros [? [? [? ?]]]; [|inversion H6;subst].
+                  + exists (Idle {| current := inr v; ticket := ticket0; owner := owner0 |}),
+    (TMap.add t0 (ls_linr (tryPlaceTask o n i) (inr v)) (TMap.add t0 (ls_lini (tryPlaceTask o n i)) x0)).
+                    apply H in H6 as HΔ'; inversion HΔ'; simpl in *; subst.
+                    simpl. split; [constructor|do 2 (rewrite TMap.gso; eauto) ]; eauto.
+                    eapply rt_trans.
+                    eapply rt_step, ps_inv; eauto.
+                    do 2 constructor.
+                    eapply rt_step, ps_ret; eauto.
+                    constructor. eapply step_tryPlaceTask_fail; eauto.
+                    rewrite TMap.gss; auto.
+                  + do 2 eexists; split; eauto.
+                    do 2 (rewrite TMap.gso; eauto).
+              }
+
+              
+            }
+            
+          }
+          intros.
+          eapply provable_ret;
+          try solve_conj_impl;
+          try solve_stable stableDB.
+          left; auto.
+        }
+      }
+    }
+
+
+End CASTaskImpl.
 
 
 Module CCASImpl.
